---
title: "Latex Test"
author: "Archisman Mukherjee"
draft: true
---

Test post with latex.

The objective of this section is to study the sum of $k$th powers of first $n$ natural numbers, that is, the sum $S_k(n) = 1^k + 2^k + 3^k + \ldots + (n-1)^k + n^k$. Clearly, $S_k(n) - S_k(n-1) = n^k$. So by the method of finite differences, but applied in reverse, we can see that $S_k(n)$ must be a $(k+1)$ degree polynomial in $n$. But what polynomial is it? Sadly, the exact expression for general $k$ is not very easy to compute, but we will present a general method. For $k = 1$ it is the sum of an AP, so pairing terms from the beginning and end works, but this doesn't work for general $k$. Instead, we will use the Binomial Theorem to get that $(k+1)$ degree polynomial:$$(n+1)^{k+1} - n^{k+1} = \binom{k+1}{1}n^k + \binom{k+1}{2}n^{k-1} + \ldots + \binom{k+1}{k+1}$$$$n^{k+1} - (n-1)^{k+1} = \binom{k+1}{1}(n-1)^k + \binom{k+1}{2}(n-1)^{k-1} + \ldots + \binom{k+1}{k+1}$$$$\cdots$$$$\bigoplus \qquad 2^{k+1} - 1^{k+1} = \binom{k+1}{1} + \binom{k+1}{2} + \ldots + \binom{k+1}{k+1}$$\hrule$$\implies (n+1)^{k+1} - 1 = \binom{k+1}{1} (1^k + 2^k + \ldots + n^k) + \binom{k+1}{2} (1^{k-1} + 2^{k-1} + \ldots + n^{k-1}) + \ldots + \binom{k+1}{k+1} (1 + 1 + \ldots + 1)$$Note how this resembles the strong form of induction. The base case $S_0(n) = 1 + 1 + \ldots + 1 = n$ is known, and to find out $S_k$, you need to know $S_0(n), S_1(n) \ldots S_{k-1}(n)$. Let us look at some small values of $k$. For $k = 1$:$$(n+1)^2 - 1 = 2S_1(n) + S_0(n) \implies n^2 + 2n = 2S_1 + n \implies \boxed{S_1 = \frac{n(n+1)}{2}}$$exactly what we got from AP. Now, for $k = 2$, (here onwards $S_k$ means $S_k(n)$ since we are not varying $n$):$$(n+1)^3 - 1 = 3S_2 + 3S_1 + S_0 \implies n^3 + 3n^2 + \cancel{3n} \text{   } 2n = 3S_2 + 3\frac{n(n+1)}{2} + \cancel{n} $$$$\implies n(n+1)(n+2) - 3\frac{n(n+1)}{2} = 3S_2 \implies \boxed{S_2 = \frac{n(n+1)(2n+1)}{6}}$$Note that each of these formulas can be verified by induction very easily.

Suppose we want to find the sum $S$ of the AGP $(a+(n-1)d)r^{n-1}$. We write:
$\displaystyle{1S = a + (a+d)r + (a+2d)r^2 + (a+3d)r^3+ \ldots + (a+(n-1)d)r^{n-1}}$
$\displaystyle{rS = 0 + (a+0)r + (a+1d)r^2 + (a+2d)r^3 + \ldots + (a+(n-2)d)r^{n-1}+ (a+(n-1)d)r^n}$

Subtracting the two equations like in case of GP, we get: $$(1-r)S = a - (a+(n-1)d)r^{n-1} + (dr + dr^2 + dr^3 + \ldots + dr^{n-1}) = a - (a+(n-1)d)r^{n-1} + dr\frac{(1-r^{n-1})}{1-r}$$If the coefficients of $r^n$ are in $k$th order AP, we simply have to repeat this process $k$ times to bring down the degree of the coefficients to $0$, at which point it becomes the usual GP